@prefix psi: <http://parliament.uk/ontologies/statutory-instrument/> . 
@prefix xsd: <http://www.w3.org/2001/XMLSchema#> . 
@prefix rdf: <http://www.w3.org/1999/02/22-rdf-syntax-ns#> .
@prefix dcterms: <http://purl.org/dc/terms/> .
@prefix owl:     <http://www.w3.org/2002/07/owl#> .
@prefix rdfs:    <http://www.w3.org/2000/01/rdf-schema#> .

<http://parliament.uk/ontologies/statutory-instrument/> 
    rdf:type owl:Ontology ;
    dcterms:title "Statutory Instrument ontology"@en ;
    dcterms:created "21/03/2018"^^xsd:date ;
	dcterms:rights "Open Parliament Licence v3.0"@en ;
    dcterms:description "Statutory Instrument ontology for UK Parliament. Needs to be read in association with the laying, tabling, procedure and core ontologies."@en .


#######  Classes ##### 	

psi:Legislation rdf:type owl:Class ;
	rdfs:label "Legislation"@en ;
	rdfs:comment "A piece of legislation. Either primary or secondary."@en ;
	rdf:isDefinedBy <http://parliament.uk/ontologies/statutory-instrument/> .
	
psi:SecondaryLegislation rdf:type owl:Class ;
	rdfs:subClassOf psi:Legislation ;
	rdfs:label "SecondaryLegislation"@en ;
	rdfs:comment "A piece of secondary legislation. Secondary legislation is also referred to as delegated legislation. The terms are synonymous. The term delegated refers to the fact that the powers claimed by the legislation are delegated from a piece of primary legislation."@en ;
	rdf:isDefinedBy <http://parliament.uk/ontologies/statutory-instrument/> .

psi:StatutoryInstrument rdf:type owl:Class ;
	rdfs:subClassOf psi:SecondaryLegislation ;
	rdfs:label "StatutoryInstrument"@en ;
	rdfs:comment "A statutory instrument"@en ;
	rdf:isDefinedBy <http://parliament.uk/ontologies/statutory-instrument/> .
	

	
##### Object properties ####


psi:enabledBy rdf:type owl:ObjectProperty ;
	rdfs:label "enabledBy"@en ;
	rdfs:comment "Relates a statutory instrument to the item of legislation or items of legislation which enable it. The enabling legislation delegates powers to the statutory instrument. Note that sometimes a statutory instrument will be enabled by another piece of secondary legislation. But that must in turn be enabled by an Act (a piece of primary legislation). IS THIS TRUE. Could it be SI > SI > SI > Act?"@en ;
	rdfs:domain psi:StatutoryInstrument ;
	rdfs:range psi:Legislation ;
	rdf:isDefinedBy <http://parliament.uk/ontologies/statutory-instrument/> .
				
	
##### Data properties ####	
			
psi:legislationURI rdf:type owl:DatatypeProperty ;
	rdfs:label "legislationURI"@en ;
	rdfs:comment "The URI of the legislation (on legislation.gov.uk)."@en ;
	rdfs:domain psi:Legislation ;
	rdfs:range rdfs:Literal ;
	rdf:isDefinedBy <http://parliament.uk/ontologies/statutory-instrument/> .
	
psi:impactAssessmentURI rdf:type owl:DatatypeProperty ;
	rdfs:label "impactAssessmentURI"@en ;
	rdfs:comment "The URI of the impact assessment associated with the legislation (on legislation.gov.uk)."@en ;
	rdfs:domain psi:Legislation ;
	rdfs:range rdfs:Literal ;
	rdf:isDefinedBy <http://parliament.uk/ontologies/statutory-instrument/> .
	
psi:explanatoryMemorandumURI rdf:type owl:DatatypeProperty ;
	rdfs:label "explanatoryMemorandumURI"@en ;
	rdfs:comment "The URI of the explanatory memorandum associated with the legislation (on legislation.gov.uk)."@en ;
	rdfs:domain psi:Legislation ;
	rdfs:range rdfs:Literal ;
	rdf:isDefinedBy <http://parliament.uk/ontologies/statutory-instrument/> .
	
psi:siNumber rdf:type owl:DatatypeProperty ;
	rdfs:label "siNumber"@en ;
	rdfs:comment "The number of the SI."@en ;
	rdfs:domain psi:StatutoryInstrument ;
	rdfs:range xsd:integer ;
	rdf:isDefinedBy <http://parliament.uk/ontologies/statutory-instrument/> .
	
psi:madeDate rdf:type owl:DatatypeProperty ;
	rdfs:label "madeDate"@en ;
	rdfs:comment "The date on which the SI was or is going to be made. Note that making happens outside of Parliament by the minister responsible for the SI."@en ;
	rdfs:domain psi:StatutoryInstrument ;
	rdfs:range xsd:date ;
	rdf:isDefinedBy <http://parliament.uk/ontologies/statutory-instrument/> .
	
psi:comingIntoForceDate rdf:type owl:DatatypeProperty ;
	rdfs:label "comingIntoForceDate"@en ;
	rdfs:comment "The date on which the SI was or is going to come into force. Where given this will be the date on which the whole SI comes into force. Sometimes coming into force will be fuzzier than a given date. Sometimes different schedules within the SI will come into force at different times. In these cases there'll be no comingIntoForceDate but the coming into force details will be given as a comingIntoForceNote."@en ;
	rdfs:domain psi:StatutoryInstrument ;
	rdfs:range xsd:date ;
	rdf:isDefinedBy <http://parliament.uk/ontologies/statutory-instrument/> .
	
psi:comingIntoForceNote rdf:type owl:DatatypeProperty ;
	rdfs:label "comingIntoForceNote"@en ;
	rdfs:comment "A note to say when the SI was or is going to come into force. Sometimes coming into force will be fuzzier than a given date. Sometimes different schedules within the SI will come into force at different times. In these cases there'll be no comingIntoForceDate but the coming into force details will be given as a comingIntoForceNote."@en ;
	rdfs:domain psi:StatutoryInstrument ;
	rdfs:range rdf:langString ;
	rdf:isDefinedBy <http://parliament.uk/ontologies/statutory-instrument/> .
						