@prefix plg: <http://parliament.uk/ontologies/legislation/> . 
@prefix xsd: <http://www.w3.org/2001/XMLSchema#> . 
@prefix rdf: <http://www.w3.org/1999/02/22-rdf-syntax-ns#> .
@prefix dcterms: <http://purl.org/dc/terms/> .
@prefix owl:     <http://www.w3.org/2002/07/owl#> .
@prefix rdfs:    <http://www.w3.org/2000/01/rdf-schema#> .

<http://parliament.uk/ontologies/legislation/> 
    rdf:type owl:Ontology ;
    dcterms:title "Legislation ontology"@en ;
    dcterms:created "21/03/2018"^^xsd:date ;
	dcterms:rights "Open Parliament Licence v3.0"@en ;
    dcterms:description "Legislation ontology for UK Parliament. Needs to be read in conjunction with the laying, tabling, procedure and core ontologies."@en .


#######  Classes ##### 	

plg:ActOfParliament rdf:type owl:Class ;
	rdfs:label "ActOfParliament"@en ;
	rdfs:comment "An Act of Parliament creates a new law or changes an existing law. Once a Bill has been approved by both the House of Commons and the House of Lords and been given Royal Assent by the Monarch it becomes an Act of Parliament. Taken together, Acts of Parliament make up what is known as Statute Law in the UK."@en ;
	rdf:isDefinedBy <http://parliament.uk/ontologies/legislation/> .
	
plg:StatutoryDayCount rdf:type owl:Class ;
	rdfs:label "StatutoryDayCount"@en ;
	rdfs:comment "Some Acts of Parliament define a day count during which Parliament may scrutinise an instrument. The days may either be sitting days or statutory days (see the time period ontology) e.g. the Statutory Instruments Act 1946 defines a default period of 40 statutory days of scrutiny for instruments subject to parliamentary procedure. Sometimes the enabling act (via enabling power) may define an exception to this default. Most commonly this will be 28, 60 or 120 days."@en ;
	rdf:isDefinedBy <http://parliament.uk/ontologies/legislation/> .

plg:StatutoryDayCountType rdf:type owl:Class ;
	rdfs:label "StatutoryDayCountType"@en ;
	rdfs:comment "Statutory day counts are calculated according to the day type specified in an Act. Sometimes only sitting days are counted. Sometimes statutory days are counted. See the time period ontology for definitions."@en ;
	rdf:isDefinedBy <http://parliament.uk/ontologies/legislation/> .

plg:EnablingPower rdf:type owl:Class ;
	rdfs:label "EnablingPower"@en ;
	rdfs:comment "A power delegated by one or more items of primary legislation, enabling a government minister to bring forward secondary legislation. The terms under which the secondary legislation can be brought forward, such as the procedure it will be subject to, any override of statutory day count, and the scope of the secondary legislation are specified by the enabling power."@en ;
	rdf:isDefinedBy <http://parliament.uk/ontologies/legislation/> .
	
plg:WorkPackage rdf:type owl:Class ;
	rdfs:label "WorkPackage"@en ;
	rdfs:comment "A package of work grouping together many individual business items e.g. the passage of a specific statutory instrument, or the passage of a specific public bill etc. Whereas a procedure (and its accompanying routes and steps) describes the process, the work package handles the application of that process for a specific instance."@en ;
	rdf:isDefinedBy <http://parliament.uk/ontologies/legislation/> .

plg:WorkPackageableThing rdf:type owl:Class ;
	rdfs:label "WorkPackageableThing"@en ;
	rdfs:comment "Any thing that can be the focus of a workpackage."@en ;
	rdf:isDefinedBy <http://parliament.uk/ontologies/legislation/> .

plg:ProposedNegativeStatutoryInstrument rdf:type owl:Class ;
	rdfs:subClassOf plg:WorkPackageableThing ;
	rdfs:subClassOf plg:StatutoryEnabledThing ;
	rdfs:label "ProposedNegativeStatutoryInstrument"@en ;
	rdfs:comment "All regulations proposed to be made under the powers in clauses 7, 8 or 9 of the European Union (Withdrawal) Bill, which Ministers consider need to be made under the negative procedure, will be laid before both Houses as proposed statutory instruments. Sifting committees in both Houses may recommend a change to the affirmative procedure. A proposed statutory instrument may lead to a statutory instrument being laid, or multiple, or none. This is subject to change given amendments made to the EU Withdrawal Bill."@en ;
	rdf:isDefinedBy <http://parliament.uk/ontologies/legislation/> .
	
plg:StatutoryEnabledThing rdf:type owl:Class ;
	rdfs:label "StatutoryEnabledThing"@en ;
	rdfs:comment "Any parliamentary thing whose existence is enabled and / or governed by statute law."@en ;
	rdf:isDefinedBy <http://parliament.uk/ontologies/legislation/> .

plg:DraftAndMadeStatutoryInstrumentSubjectToParliamentaryProcedure rdf:type owl:Class ;
	rdfs:subClassOf plg:WorkPackageableThing ;
	rdfs:subClassOf plg:StatutoryEnabledThing ;
	rdfs:label "DraftAndMadeStatutoryInstrumentSubjectToParliamentaryProcedure"@en ;
	rdfs:comment "Both draft and made statutory instruments are subject to parliamentary procedure. See the procedure ontology for details. This is at a higher conceptual level than the FRBR work identified by legislation.gov.uk and provides a way to abstract away from their document based model to things that Parliament takes an interest in."@en ;
	rdf:isDefinedBy <http://parliament.uk/ontologies/legislation/> .

plg:DraftStatutoryInstrument rdf:type owl:Class ;
	rdfs:label "DraftStatutoryInstrument"@en ;
	rdfs:comment "A draft statutory instrument. Subject to parliamentary approval, this can become an item of secondary legislation if and when a government minister 'makes' it. Despite not (yet) being legislation, draft statutory instruments are published on legislation.gov.uk. Equivalent to a FRBR work in a legislation.gov.uk sense."@en ;
	rdf:isDefinedBy <http://parliament.uk/ontologies/legislation/> .

plg:MadeStatutoryInstrument rdf:type owl:Class ;
	rdfs:label "MadeStatutoryInstrument"@en ;
	rdfs:comment "A statutory instrument which has been made into law by a government minister. Statutory instruments are a type of secondary (or delegated) legislation. They can be used to make specific changes to the law under enabling powers delegated by Acts of Parliament."@en ;
	rdf:isDefinedBy <http://parliament.uk/ontologies/legislation/> .
	

##### Object properties ####

plg:delegates rdf:type owl:ObjectProperty ;
	rdfs:label "delegates"@en ;
	rdfs:comment "Relates an Act of Parliament to an enabling power delegated by that Act. Secondary legislation can also delegate powers to make further subordinate legislation. This is known as a sub-delegation or tertiary law. Such law is not usually made by statutory instrument, and doesnâ€™t come near Parliament."@en ;
	rdfs:domain plg:ActOfParliament ;
	rdfs:range plg:EnablingPower ;
	rdf:isDefinedBy <http://parliament.uk/ontologies/legislation/> .

plg:specifiesStatutoryDayCount rdf:type owl:ObjectProperty ;
	rdfs:label "specifiesStatutoryDayCount"@en ;
	rdfs:comment "Relates an Act of Parliament to a statutory day count. For statutory instruments the default statutory day count is 40 statutory days as defined by the Statutory Instruments Act 1946. Sometimes the enabling Act will override this value."@en ;
	rdfs:domain plg:ActOfParliament ;
	rdfs:range plg:StatutoryDayCount ;
	rdf:isDefinedBy <http://parliament.uk/ontologies/legislation/> .
	
plg:dayType rdf:type owl:ObjectProperty ;
	rdfs:label "dayType"@en ;
	rdfs:comment "Relates a statutory day count to a statutory day count type. Values might be sitting days or statutory days. See the time period ontology for definitions."@en ;
	rdfs:domain plg:StatutoryDayCount ;
	rdfs:range plg:StatutoryDayCountType ;
	rdf:isDefinedBy <http://parliament.uk/ontologies/legislation/> .
	
plg:dayCountDefinedBy rdf:type owl:ObjectProperty ;
	rdfs:label "dayCountDefinedBy"@en ;
	rdfs:comment "Relates a work package to a statutory day count."@en ;
	rdfs:domain plg:WorkPackage ;
	rdfs:range plg:StatutoryDayCount ;
	rdf:isDefinedBy <http://parliament.uk/ontologies/legislation/> .
	
plg:focus rdf:type owl:ObjectProperty ;
	rdfs:label "focus"@en ;
	rdfs:comment "Relates a work package to a work packageable thing."@en ;
	rdfs:domain plg:WorkPackage ;
	rdfs:range plg:WorkPackageableThing ;
	rdf:isDefinedBy <http://parliament.uk/ontologies/legislation/> .
	
plg:enabledBy rdf:type owl:ObjectProperty ;
	rdfs:label "enabledBy"@en ;
	rdfs:comment "Relates a statutory enabled thing to the power that enables it. Statutory instruments have an enabling power derived from one or more Acts of Parliament."@en ;
	rdfs:domain plg:StatutoryEnabledThing ;
	rdfs:range plg:EnablingPower ;
	rdf:isDefinedBy <http://parliament.uk/ontologies/legislation/> .
	
plg:precededByProposedNegativeStatutoryInstrument rdf:type owl:ObjectProperty ;
	rdfs:label "precededByProposedNegativeStatutoryInstrument"@en ;
	rdfs:comment "Relates a draft or made statutory instrument subject to parliamentary procedure to any preceding proposed negative statutory instrument(s)."@en ;
	rdfs:domain plg:DraftAndMadeStatutoryInstrumentSubjectToParliamentaryProcedure ;
	rdfs:range plg:ProposedNegativeStatutoryInstrument ;
	rdf:isDefinedBy <http://parliament.uk/ontologies/legislation/> .
	
plg:embodiedAsDraftStatutoryInstrument rdf:type owl:ObjectProperty ;
	rdfs:label "embodiedAsDraftStatutoryInstrument"@en ;
	rdfs:comment "Relates a draft or made statutory instrument subject to parliamentary procedure to the FRBR work level of any document published on legislation.gov.uk in draft form."@en ;
	rdfs:domain plg:DraftAndMadeStatutoryInstrumentSubjectToParliamentaryProcedure ;
	rdfs:range plg:DraftStatutoryInstrument ;
	rdf:isDefinedBy <http://parliament.uk/ontologies/legislation/> .
	
plg:embodiedAsMadeStatutoryInstrument rdf:type owl:ObjectProperty ;
	rdfs:label "embodiedAsMadeStatutoryInstrument"@en ;
	rdfs:comment "Relates a draft or made Statutory Instrument subject to parliamentary procedure to the FRBR work level of any document published on legislation.gov.uk in made form."@en ;
	rdfs:domain plg:DraftAndMadeStatutoryInstrumentSubjectToParliamentaryProcedure ;
	rdfs:range plg:MadeStatutoryInstrument ;
	rdf:isDefinedBy <http://parliament.uk/ontologies/legislation/> .
				
	
##### Data properties ####	
			
plg:count rdf:type owl:DatatypeProperty ;
	rdfs:label "count"@en ;
	rdfs:comment "Specifies the total number of days of a given type. This is the period during which a statutory instrument or proposed negative statutory instrument is subject to parliamentary scrutiny."@en ;
	rdfs:domain plg:StatutoryDayCount ;
	rdfs:range xsd:integer ;
	rdf:isDefinedBy <http://parliament.uk/ontologies/legislation/> .

plg:siPrefix rdf:type owl:DatatypeProperty ;
	rdfs:label "siPrefix"@en ;
	rdfs:comment "The prefix of a statutory instrument. Usually this will be SI. Other prefixes, such as for regulations include SR (NI). The prefix forms the first part of the standard citation 'number' for a statutory instrument e.g. SI 1986/925."@en ;
	rdfs:domain plg:DraftAndMadeStatutoryInstrumentSubjectToParliamentaryProcedure ;
	rdfs:range rdfs:Literal ;
	rdf:isDefinedBy <http://parliament.uk/ontologies/legislation/> .
	
plg:siYear rdf:type owl:DatatypeProperty ;
	rdfs:label "siYear"@en ;
	rdfs:comment "The year of a statutory instrument. Usually this will be the year it was laid before Parliament. Occasionally a statutory instrument laid in draft in one calendar year and made the following calendar year will have its SI year updated. The year forms the second part of the standard citation 'number' for a statutory instrument e.g. SI 1986/925."@en ;
	rdfs:domain plg:DraftAndMadeStatutoryInstrumentSubjectToParliamentaryProcedure ;
	rdfs:range xsd:integer ;
	rdf:isDefinedBy <http://parliament.uk/ontologies/legislation/> .
	
plg:siNumberInYear rdf:type owl:DatatypeProperty ;
	rdfs:label "siNumberInYear"@en ;
	rdfs:comment "Statutory instruments are given a number in a year (see siYear). The number forms the third part of the standard citation 'number' for a statutory instrument e.g. SI 1986/925."@en ;
	rdfs:domain plg:DraftAndMadeStatutoryInstrumentSubjectToParliamentaryProcedure ;
	rdfs:range xsd:integer ;
	rdf:isDefinedBy <http://parliament.uk/ontologies/legislation/> .
	
plg:madeDate rdf:type owl:DatatypeProperty ;
	rdfs:label "madeDate"@en ;
	rdfs:comment "The date on which the statutory instrument was made. Note that the process of making happens outside Parliament, by the minister responsible for the statutory instrument."@en ;
	rdfs:domain plg:DraftAndMadeStatutoryInstrumentSubjectToParliamentaryProcedure ;
	rdfs:range xsd:date ;
	rdf:isDefinedBy <http://parliament.uk/ontologies/legislation/> .
	
plg:comingIntoForceDate rdf:type owl:DatatypeProperty ;
	rdfs:label "comingIntoForceDate"@en ;
	rdfs:comment "The date on which the statutory instrument came, or is going to come, into force. Where given, this will be the date on which the whole statutory instrument comes into force. Sometimes coming into force will be fuzzier than a given date e.g. different schedules within the SI will come into force at different times. In these cases there'll be no comingIntoForceDate; the coming into force details will be given as a comingIntoForceNote."@en ;
	rdfs:domain plg:DraftAndMadeStatutoryInstrumentSubjectToParliamentaryProcedure ;
	rdfs:range xsd:date ;
	rdf:isDefinedBy <http://parliament.uk/ontologies/legislation/> .
	
plg:comingIntoForceNote rdf:type owl:DatatypeProperty ;
	rdfs:label "comingIntoForceNote"@en ;
	rdfs:comment "A note to say when the statutory instrument came, or is going to come, into force. Sometimes coming into force will be fuzzier than a given date e.g. different schedules within the SI will come into force at different times. In these cases there'll be no comingIntoForceDate but the coming into force details will be given as a comingIntoForceNote."@en ;
	rdfs:domain plg:DraftAndMadeStatutoryInstrumentSubjectToParliamentaryProcedure ;
	rdfs:range rdf:langString ;
	rdf:isDefinedBy <http://parliament.uk/ontologies/legislation/> .
						