@prefix ppr: <http://parliament.uk/ontologies/procedure/> . 
@prefix xsd: <http://www.w3.org/2001/XMLSchema#> . 
@prefix rdf: <http://www.w3.org/1999/02/22-rdf-syntax-ns#> .
@prefix dcterms: <http://purl.org/dc/terms/> .
@prefix owl:     <http://www.w3.org/2002/07/owl#> .
@prefix rdfs:    <http://www.w3.org/2000/01/rdf-schema#> .
@prefix foaf:	<http://xmlns.com/foaf/0.1/> .

<http://parliament.uk/ontologies/procedure/> 
    rdf:type owl:Ontology ;
    dcterms:title "Procedure ontology"@en ;
    dcterms:created "20/02/2018"^^xsd:date ;
	dcterms:rights "Open Parliament Licence v3.0"@en ;
    dcterms:description "Procedure ontology for UK Parliament. An abstract ontology for describing how process steps or stages can be combined into a procedure."@en ;
	dcterms:author <http://smethur.st/#me> ;
	foaf:depiction <procedure.png>
	foaf:maker
		[ foaf:name "David Beamish" ],
		[ foaf:name "Robert Brook" ],
		[ foaf:name "Jack Dent" ],
		[ foaf:name "Silver Oliver" ],
		[ foaf:name "Michael Smethurst"; foaf:homepage <http://smethur.st/> ],
	    [ foaf:name "Anya Somerville" ]
		[ foaf:name "Jane White" ] .


#######  Classes #####

ppr:Step rdf:type owl:Class ;
	rdfs:label "Step"@en ;
	rdfs:comment "A step in a procedure e.g. consideration of a statutory instrument by the Joint Committee on Statutory Instruments. Steps may not be unique to a specific procedure e.g. the consideration described happens in both the affirmative and negative statutory instrument procedure."@en ;
	rdfs:isDefinedBy <http://parliament.uk/ontologies/procedure/> .
	
ppr:Route rdf:type owl:Class ;
	rdfs:label "Route"@en ;
	rdfs:comment "Links a procedural step or steps, according to the RouteType. Routes are time bound, using startOn and endOn from the Core Ontology. This allows routes to reflect changes in procedure. A route is activated once the preceding steps are actualised by a business item. Some steps only occur once in a work package: the RouteType with the name 'precludes' can route an actualised step to itself. This precludes any further instances of that step in the work package e.g. in the made affirmative statutory instrument procedure the step 'cleared by the Joint Committee on Statutory Instruments' can happen only once."@en ;
	rdfs:isDefinedBy <http://parliament.uk/ontologies/procedure/> .
	
ppr:RouteType rdf:type owl:Class ;
	rdfs:label "RouteType"@en ;
	rdfs:comment "Route types are: causes, allows, precludes and requires. A route of type 'causes' relates the route to a following step where completion of the preceding step(s) directly causes the route to trigger the next step i.e. the next step is inevitable. A route of type 'allows' relates the route to a following step where completion of the preceding step(s) allows the next step to happen, but does not cause it to happen i.e. the next step might happen but is not inevitable. A route of type 'precludes' relates a route to a step where completion of the preceding step(s) precludes that step from happening i.e. the next step can no longer happen. A route of type 'requires' relates a route to a step where completion of the preceding step(s) is required before that step can happen i.e. the next step can't happen unless the preceding step has been completed."@en ;
	rdfs:isDefinedBy <http://parliament.uk/ontologies/procedure/> .
	
ppr:House rdf:type owl:Class ;
	rdfs:label "House"@en ;
	rdfs:comment "A parliamentary House e.g. the House of Lords."@en ;
	rdfs:isDefinedBy <http://parliament.uk/ontologies/procedure/> .
	
ppr:Procedure rdf:type owl:Class ;
	rdfs:label "Procedure"@en ;
	rdfs:comment "A parliamentary procedure in a particular House or Houses. An example might be the passage of a made affirmative statutory instrument in both Houses. Note that some procedures are House specific, but can involve things like a joint committee that cuts across the two Houses. In the latter case we consider it to be a single procedure."@en ;
	rdfs:isDefinedBy <http://parliament.uk/ontologies/procedure/> .
	
ppr:BusinessItem rdf:type owl:Class ;
	rdfs:label "BusinessItem"@en ;
	rdfs:comment "An item of parliamentary business e.g. a second reading debate, the tabling of an early day motion, a laying of a paper."@en ;
	rdfs:isDefinedBy <http://parliament.uk/ontologies/procedure/> .
	
ppr:WorkPackage rdf:type owl:Class ;
	rdfs:label "WorkPackage"@en ;
	rdfs:comment "A package of work grouping together individual business items e.g. the passage of a specific statutory instrument, or the passage of a specific public bill. Whereas a procedure and its accompanying routes and steps describes the process, the work package and its business items handles the application of that process on a specific work packageable thing."@en ;
	rdfs:isDefinedBy <http://parliament.uk/ontologies/procedure/> .
	
ppr:WorkPackageableThing rdf:type owl:Class ;
	rdfs:label "WorkPackageableThing"@en ;
	rdfs:comment "Any thing that can be the focus of a work package e.g. a statutory instrument, a public bill, a committee inquiry."@en ;
	rdfs:isDefinedBy <http://parliament.uk/ontologies/procedure/> .
	
#######  Object properties ##### 

ppr:belongsTo rdf:type owl:ObjectProperty ;
	rdfs:label "belongsTo"@en ;
	rdfs:comment "Relates an individual business item to the work package it is part of. Note that whilst a work package can contain many business items, a business item might relate to several work packages e.g. a meeting of the Joint Committee on Statutory Instruments might include business relating to many SI work packages with no distinct segmentation. Note also that the ordering of business items in a work package cannot be determined by the (end) date alone. Many business items inside a work package may share the same (end) date. In this case ordinality can only be determined by spanning the procedure tree, taking into account actualised steps and the route types joining steps to determine the real-world order."@en ;
	rdfs:domain ppr:BusinessItem ;
	rdfs:range ppr:WorkPackage ;
	rdfs:isDefinedBy <http://parliament.uk/ontologies/procedure/> .
	
ppr:subjectTo rdf:type owl:ObjectProperty ;
	rdfs:label "subjectTo"@en ;
	rdfs:comment "Relates a work packageable thing to the procedure it is subject to. A work packageable thing can only be subject to one procedure."@en ;
	rdfs:domain ppr:WorkPackageableThing ;
	rdfs:range ppr:Procedure ;
	rdfs:isDefinedBy <http://parliament.uk/ontologies/procedure/> .
	
ppr:actualises rdf:type owl:ObjectProperty ;
	rdfs:label "actualises"@en ;
	rdfs:comment "Relates a business item to a step in a procedure (via a route) e.g. relates the second reading of a specific public bill to the corresponding (conceptual) step in the procedure. Note that whilst a step might be actualised by several business items (in different work packages), a business item might actualise one or several steps e.g. there might be a calendarised business item on the order paper that includes a debate on a number of motions. This would actualise steps relating each of those motions."@en ;
	rdfs:domain ppr:BusinessItem ;
	rdfs:range ppr:Step ;
	rdfs:isDefinedBy <http://parliament.uk/ontologies/procedure/> .

ppr:fromStep rdf:type owl:ObjectProperty ;
	rdfs:label "fromStep"@en ;
	rdfs:comment "Relates a route to a preceding step."@en ;
	rdfs:domain ppr:Route ;
	rdfs:range ppr:Step ;
	rdfs:isDefinedBy <http://parliament.uk/ontologies/procedure/> .
	
ppr:toStep rdf:type owl:ObjectProperty ;
	rdfs:label "toStep"@en ;
	rdfs:comment "Relates a route to a potential following step. Note that the 'next' step might be precluded by the route type."@en ;
	rdfs:domain ppr:Route ;
	rdfs:range ppr:Step ;
	rdfs:isDefinedBy <http://parliament.uk/ontologies/procedure/> .
	
ppr:hasRouteType rdf:type owl:ObjectProperty ;
	rdfs:label "hasRouteType"@en ;
	rdfs:comment "Relates a route to a route type. A route can have one only type."@en ;
	rdfs:domain ppr:Route ;
	rdfs:range ppr:RouteType ;
	rdfs:isDefinedBy <http://parliament.uk/ontologies/procedure/> .
	
ppr:follows rdf:type owl:ObjectProperty ;
	rdfs:label "follows"@en ;
	rdfs:comment "Relates a procedure to a route. A route can belong to only one procedure."@en ;
	rdfs:domain ppr:Procedure ;
	rdfs:range ppr:Route ;
	rdfs:isDefinedBy <http://parliament.uk/ontologies/procedure/> .
	
ppr:stepInHouse rdf:type owl:ObjectProperty ;
	rdfs:label "stepInHouse"@en ;
	rdfs:comment "Relates a step to one or both Houses."@en ;
	rdfs:domain ppr:Step ;
	rdfs:range ppr:House ;
	rdfs:isDefinedBy <http://parliament.uk/ontologies/procedure/> .
		
ppr:procedureInHouse rdf:type owl:ObjectProperty ;
	rdfs:label "procedureInHouse"@en ;
	rdfs:comment "Relates a procedure to one or both Houses."@en ;
	rdfs:domain ppr:Procedure ;
	rdfs:range ppr:House ;
	rdfs:isDefinedBy <http://parliament.uk/ontologies/procedure/> .
		
ppr:focus rdf:type owl:ObjectProperty ;
	rdfs:label "focus"@en ;
	rdfs:comment "Relates a work package to a workpackageable thing."@en ;
	rdfs:domain ppr:WorkPackage ;
	rdfs:range ppr:WorkPackageableThing ;
	rdfs:isDefinedBy <http://parliament.uk/ontologies/procedure/> .