@prefix ppr: <http://parliament.uk/ontologies/procedure/> . 
@prefix xsd: <http://www.w3.org/2001/XMLSchema#> . 
@prefix rdf: <http://www.w3.org/1999/02/22-rdf-syntax-ns#> .
@prefix dcterms: <http://purl.org/dc/terms/> .
@prefix owl:     <http://www.w3.org/2002/07/owl#> .
@prefix rdfs:    <http://www.w3.org/2000/01/rdf-schema#> .

<http://parliament.uk/ontologies/laying/> 
    rdf:type owl:Ontology ;
    dcterms:title "Procedure ontology"@en ;
    dcterms:created "20/02/2018"^^xsd:date ;
	dcterms:rights "Open Parliament Licence v3.0"@en ;
    dcterms:description "Procedure ontology for UK Parliament. An abstract ontology for describing how process steps or stages can be combined into a procedure."@en .


#######  Classes #####

ppr:Step rdf:type owl:Class ;
	rdfs:label "Step"@en ;
	rdfs:comment "A step in a procedure e.g. consideration of a statutory instrument by the Joint Committee on Statutory Instruments. Steps may not be unique to a specific procedure e.g. the consideration described in the previous example happens in both the affirmative and negative statutory instrument procedure."@en ;
	rdf:isDefinedBy <http://parliament.uk/ontologies/procedure/> .
	
ppr:Route rdf:type owl:Class ;
	rdfs:label "Route"@en ;
	rdfs:comment "Ties a procedural step to the subsequent step or steps according to the parliamentary procedure which applies. Note that routes are time bound (borrowing startOn and endOn from the Core Ontology). This allows routes to change over time and adapt to changes in procedure."@en ;
	rdf:isDefinedBy <http://parliament.uk/ontologies/procedure/> .
	
ppr:RouteType rdf:type owl:Class ;
	rdfs:label "RouteType"@en ;
	rdfs:comment "Route types are: causes, allows and precludes. A route of type 'causes' relates the route to a following step where completion of the preceding step(s) directly causes the route to trigger the next step i.e. the next step is inevitable. A route of type 'allows' relates the route to a following step where completion of the preceding step(s) allows the next step to happen, but does not cause it to happen i.e. the next step might happen but is not inevitable. A route of type 'precludes' relates a route to a step where completion of the preceding step(s) precludes that step from happening i.e. the next step can no longer happen."@en ;
	rdf:isDefinedBy <http://parliament.uk/ontologies/procedure/> .
	
ppr:House rdf:type owl:Class ;
	rdfs:label "House"@en ;
	rdfs:comment "A parliamentary House e.g. the House of Lords."@en ;
	rdf:isDefinedBy <http://parliament.uk/ontologies/procedure/> .
	
ppr:Procedure rdf:type owl:Class ;
	rdfs:label "Procedure"@en ;
	rdfs:comment "A parliamentary procedure in a particular House or Houses. An example might be the passage of an affirmative SI in both Houses. Note that some procedures are House specific, but can involve things like a joint committee that cuts across the two Houses. In this case we consider it to be a single procedure."@en ;
	rdf:isDefinedBy <http://parliament.uk/ontologies/procedure/> .
	
ppr:BusinessItem rdf:type owl:Class ;
	rdfs:label "BusinessItem"@en ;
	rdfs:comment "An item of parliamentary business."@en ;
	rdf:isDefinedBy <http://parliament.uk/ontologies/procedure/> .
	
ppr:BusinessItem rdf:type owl:Class ;
	rdfs:label "BusinessItem"@en ;
	rdfs:comment "An item of parliamentary business. The business item might be scheduled for a time and place via a calendar business item (e.g. a second reading debate), or it might not yet be scheduled (e.g. an early day motion), or it might be an item of business that is never scheduled (e.g. a written question)."@en ;
	rdf:isDefinedBy <http://parliament.uk/ontologies/procedure/> .
	
ppr:CalendarBusinessItem rdf:type owl:Class ;
	rdfs:label "CalendarBusinessItem"@en ;
	rdfs:comment "Handles the scheduling of a parliamentary business item once it has been timetabled into a calendar. The calendar business item only handles the timetabling of day, time and location and does not describe the nature of the business item."@en ;
	rdf:isDefinedBy <http://parliament.uk/ontologies/procedure/> .
	
ppr:WorkPackage rdf:type owl:Class ;
	rdfs:label "WorkPackage"@en ;
	rdfs:comment "A package of work grouping together many individual business items e.g. the passage of a specific statutory instrument or the passage of a specific public bill etc. Whereas a procedure (and its accompanying routes and steps) describes the process, the work package handles the application of that process for a specific instance."@en ;
	rdf:isDefinedBy <http://parliament.uk/ontologies/procedure/> .
	
#######  Object properties ##### 

ppr:belongsTo rdf:type owl:ObjectProperty ;
	rdfs:label "belongsTo"@en ;
	rdfs:comment "Relates an individual business item to the work package it is part of."@en ;
	rdfs:domain ppr:BusinessItem ;
	rdfs:range ppr:WorkPackage ;
	rdf:isDefinedBy <http://parliament.uk/ontologies/procedure/> .
	
ppr:calendarises rdf:type owl:ObjectProperty ;
	rdfs:label "calendarises"@en ;
	rdfs:comment "Relates a calender business item to a business item."@en ;
	rdfs:domain ppr:CalendarBusinessItem ;
	rdfs:range ppr:BusinessItem ;
	rdf:isDefinedBy <http://parliament.uk/ontologies/procedure/> .
	
ppr:subjectTo rdf:type owl:ObjectProperty ;
	rdfs:label "subjectTo"@en ;
	rdfs:comment "Relates a work package to the procedure it is subject to."@en ;
	rdfs:domain ppr:WorkPackage ;
	rdfs:range ppr:Procedure ;
	rdf:isDefinedBy <http://parliament.uk/ontologies/procedure/> .
	
ppr:actualises rdf:type owl:ObjectProperty ;
	rdfs:label "actualises"@en ;
	rdfs:comment "Relates a business item to a step in a procedure e.g. relates the second reading of a specific public bill to the corresponding (conceptual) step in the procedure."@en ;
	rdfs:domain ppr:BusinessItem ;
	rdfs:range ppr:Step ;
	rdf:isDefinedBy <http://parliament.uk/ontologies/procedure/> .

ppr:fromStep rdf:type owl:ObjectProperty ;
	rdfs:label "fromStep"@en ;
	rdfs:comment "Relates a route to a preceding step."@en ;
	rdfs:domain ppr:Route ;
	rdfs:range ppr:Step ;
	rdf:isDefinedBy <http://parliament.uk/ontologies/procedure/> .
	
ppr:toStep rdf:type owl:ObjectProperty ;
	rdfs:label "toStep"@en ;
	rdfs:comment "Relates a route to a potential following step. Note that the next step might be precluded by the route type."@en ;
	rdfs:domain ppr:Route ;
	rdfs:range ppr:Step ;
	rdf:isDefinedBy <http://parliament.uk/ontologies/procedure/> .
	
ppr:hasRouteType rdf:type owl:ObjectProperty ;
	rdfs:label "hasRouteType"@en ;
	rdfs:comment "Relates a route to a route type."@en ;
	rdfs:domain ppr:Route ;
	rdfs:range ppr:RouteType ;
	rdf:isDefinedBy <http://parliament.uk/ontologies/procedure/> .
	
ppr:follows rdf:type owl:ObjectProperty ;
	rdfs:label "follows"@en ;
	rdfs:comment "Relates a procedure to a route."@en ;
	rdfs:domain ppr:Procedure ;
	rdfs:range ppr:Route ;
	rdf:isDefinedBy <http://parliament.uk/ontologies/procedure/> .
	
ppr:in rdf:type owl:ObjectProperty ;
	rdfs:label "in"@en ;
	rdfs:comment "Relates a procedure to one or both Houses."@en ;
	rdfs:domain ppr:Procedure ;
	rdfs:range ppr:House ;
	rdf:isDefinedBy <http://parliament.uk/ontologies/procedure/> .
				

#######  Data properties ##### 

ppr:canSpawnMultiple rdf:type owl:DatatypeProperty ;
	rdfs:label "canSpawnMultiple"@en ;
	rdfs:comment "Determines if multiple instances of the step can be spawned in parallel e.g. the tabling of more than one non-fatal motion on a negative statutory instrument."@en ;
	rdfs:domain ppr:Step ;
	rdfs:range xsd:boolean ;
	rdf:isDefinedBy <http://parliament.uk/ontologies/procedure/> .	
