@prefix ppr: <http://parliament.uk/ontologies/procedure/> . 
@prefix xsd: <http://www.w3.org/2001/XMLSchema#> . 
@prefix rdf: <http://www.w3.org/1999/02/22-rdf-syntax-ns#> .
@prefix dcterms: <http://purl.org/dc/terms/> .
@prefix owl:     <http://www.w3.org/2002/07/owl#> .
@prefix rdfs:    <http://www.w3.org/2000/01/rdf-schema#> .

<http://parliament.uk/ontologies/laying/> 
    rdf:type owl:Ontology ;
    dcterms:title "Procedure ontology"@en ;
    dcterms:created "20/02/2018"^^xsd:date ;
	dcterms:rights "Open Parliament Licence v3.0"@en ;
    dcterms:description "Procedure ontology for UK Parliament. An abstract ontology for describing how process steps or stages can be combined into a procedure."@en .


#######  Classes #####

ppr:Step rdf:type owl:Class ;
	rdfs:label "Step"@en ;
	rdfs:comment "A step in a process. May occur in one or many routes."@en ;
	rdf:isDefinedBy <http://parliament.uk/ontologies/procedure/> .
	
ppr:Route rdf:type owl:Class ;
	rdfs:label "Route"@en ;
	rdfs:comment "Ties a preceding step to a following step depending on applicable procedure, point in time and conditional inputs from the preceding step. Note that routes are time bound (borrowing startOn and endOn from the Core Ontology) allowing for routes to change over time and reflect changes to procedure."@en ;
	rdf:isDefinedBy <http://parliament.uk/ontologies/procedure/> .
	
ppr:RouteLogic rdf:type owl:Class ;
	rdfs:label "RouteLogic"@en ;
	rdfs:comment "Works something like a logic gate. Route logic allows for the specification of the logic which determines a route's actions. Takes into account the completion of all preceding steps leading to the route and states whether all preceding steps must be completed (AND) or just some (OR)."@en ;
	rdf:isDefinedBy <http://parliament.uk/ontologies/procedure/> .
	
ppr:House rdf:type owl:Class ;
	rdfs:label "House"@en ;
	rdfs:comment "A parliamentary House e.g. the House of Lords."@en ;
	rdf:isDefinedBy <http://parliament.uk/ontologies/procedure/> .
	
ppr:Procedure rdf:type owl:Class ;
	rdfs:label "Procedure"@en ;
	rdfs:comment "A parliamentary procedure in a particular House. Examples might be the passage of an affirmative SI in the House of Commons, the passage of a public bill in the House of Lords etc."@en ;
	rdf:isDefinedBy <http://parliament.uk/ontologies/procedure/> .
	
ppr:BusinessItem rdf:type owl:Class ;
	rdfs:label "BusinessItem"@en ;
	rdfs:comment "An item of parliamentary business."@en ;
	rdf:isDefinedBy <http://parliament.uk/ontologies/procedure/> .
	
ppr:BusinessItem rdf:type owl:Class ;
	rdfs:label "BusinessItem"@en ;
	rdfs:comment "An item of parliamentary business."@en ;
	rdf:isDefinedBy <http://parliament.uk/ontologies/procedure/> .
	
ppr:CalendarBusinessItem rdf:type owl:Class ;
	rdfs:label "CalendarBusinessItem"@en ;
	rdfs:comment "An item of parliamentary business which has been timetabled onto a calendar."@en ;
	rdf:isDefinedBy <http://parliament.uk/ontologies/procedure/> .
	
ppr:WorkPackage rdf:type owl:Class ;
	rdfs:label "WorkPackage"@en ;
	rdfs:comment "A package of work involving many individual business items. Might be the passage of a specific statutory instrument or the passage of a specific public bill etc."@en ;
	rdf:isDefinedBy <http://parliament.uk/ontologies/procedure/> .
	
ppr:WorkPackageType rdf:type owl:Class ;
	rdfs:label "WorkPackageType"@en ;
	rdfs:comment "A type of a work package. Might be the passage of affirmative statutory instruments or the passage of public bills etc."@en ;
	rdf:isDefinedBy <http://parliament.uk/ontologies/procedure/> .
	
#######  Object properties ##### 

ppr:hasWorkPackageType rdf:type owl:ObjectProperty ;
	rdfs:label "hasWorkPackageType"@en ;
	rdfs:comment "Relates a work package to the type of work being undertaken."@en ;
	rdfs:domain ppr:WorkPackage ;
	rdfs:range ppr:WorkPackageType ;
	rdf:isDefinedBy <http://parliament.uk/ontologies/procedure/> .
	
ppr:undertakes rdf:type owl:ObjectProperty ;
	rdfs:label "undertakes"@en ;
	rdfs:comment "Relates a work package to the individual business items that comprise it."@en ;
	rdfs:domain ppr:WorkPackage ;
	rdfs:range ppr:BusinessItem ;
	rdf:isDefinedBy <http://parliament.uk/ontologies/procedure/> .
	
ppr:calendarises rdf:type owl:ObjectProperty ;
	rdfs:label "calendarises"@en ;
	rdfs:comment "Relates a calender business item to a business item."@en ;
	rdfs:domain ppr:CalendarBusinessItem ;
	rdfs:range ppr:BusinessItem ;
	rdf:isDefinedBy <http://parliament.uk/ontologies/procedure/> .
	
ppr:subjectTo rdf:type owl:ObjectProperty ;
	rdfs:label "subjectTo"@en ;
	rdfs:comment "Relates a work package type to the procedure it is subject to."@en ;
	rdfs:domain ppr:WorkPackageType ;
	rdfs:range ppr:Procedure ;
	rdf:isDefinedBy <http://parliament.uk/ontologies/procedure/> .
	
ppr:actualises rdf:type owl:ObjectProperty ;
	rdfs:label "actualises"@en ;
	rdfs:comment "Relates a business item to a step in a procedure."@en ;
	rdfs:domain ppr:BusinessItem ;
	rdfs:range ppr:Step ;
	rdf:isDefinedBy <http://parliament.uk/ontologies/procedure/> .

ppr:leadsTo rdf:type owl:ObjectProperty ;
	rdfs:label "leadsTo"@en ;
	rdfs:comment "Relates a step to a following route."@en ;
	rdfs:domain ppr:Step ;
	rdfs:range ppr:Route ;
	rdf:isDefinedBy <http://parliament.uk/ontologies/procedure/> .

ppr:causes rdf:type owl:ObjectProperty ;
	rdfs:label "causes"@en ;
	rdfs:comment "Relates a route to a following step where completion of the preceding step(s) directly causes the route to trigger the next step."@en ;
	rdfs:domain ppr:Route ;
	rdfs:range ppr:Step ;
	rdf:isDefinedBy <http://parliament.uk/ontologies/procedure/> .
	
ppr:allows rdf:type owl:ObjectProperty ;
	rdfs:label "allows"@en ;
	rdfs:comment "Relates a route to a following step where completion of the preceding step(s) allows the next step to happen, but does not cause it to happen."@en ;
	rdfs:domain ppr:Route ;
	rdfs:range ppr:Step ;
	rdf:isDefinedBy <http://parliament.uk/ontologies/procedure/> .
	
ppr:applies rdf:type owl:ObjectProperty ;
	rdfs:label "applies"@en ;
	rdfs:comment "Relates a route to the route logic applied."@en ;
	rdfs:domain ppr:Route ;
	rdfs:range ppr:RouteLogic ;
	rdf:isDefinedBy <http://parliament.uk/ontologies/procedure/> .
	
ppr:follows rdf:type owl:ObjectProperty ;
	rdfs:label "follows"@en ;
	rdfs:comment "Relates a procedure to a route."@en ;
	rdfs:domain ppr:Procedure ;
	rdfs:range ppr:Route ;
	rdf:isDefinedBy <http://parliament.uk/ontologies/procedure/> .
	
ppr:in rdf:type owl:ObjectProperty ;
	rdfs:label "in"@en ;
	rdfs:comment "Relates a procedure to a House."@en ;
	rdfs:domain ppr:Procedure ;
	rdfs:range ppr:House ;
	rdf:isDefinedBy <http://parliament.uk/ontologies/procedure/> .
				

#######  Data properties ##### 

ppr:canSpawnMultiple rdf:type owl:DatatypeProperty ;
	rdfs:label "canSpawnMultiple"@en ;
	rdfs:comment "Determines if multiple versions of the step can be spawned in parallel. Or just one."@en ;
	rdfs:domain ppr:Step ;
	rdfs:range xsd:boolean ;
	rdf:isDefinedBy <http://parliament.uk/ontologies/procedure/> .	
